TPTP/CNF/Parse.lean
@@ -20,10 +20,16 @@ namespace TPTP.CNF
 open Grip GParser
 open TPTP.FirstOrder.Parser
 
-private def positiveLiteral : P Literal :=
+private
+def positiveLiteral
+    : P Literal
+    :=
   Literal.positive <$> FirstOrder.Parser.atom
 
-private def parenthesizedAtom : P FirstOrder.Atom :=
+private
+def parenthesizedAtom
+    : P FirstOrder.Atom
+    :=
   GParser.ch '(' *> trivia *> FirstOrder.Parser.atom <* GParser.ch ')' <* trivia
 
 private def negativeLiteral : P Literal := gdo
@@ -33,12 +39,18 @@ private def negativeLiteral : P Literal := gdo
   return .negative value
   grade_by by decide
 
-private def literal : P Literal :=
+private
+def literal
+    : P Literal
+    :=
   GParser.dispatch fun byte =>
     if byte == Ascii.code '~' then negativeLiteral
     else positiveLiteral
 
-private def separator : P Unit :=
+private
+def separator
+    : P Unit
+    :=
   (fun _ => ()) <$> (GParser.ch '|' <* trivia)
 
 private
@@ -54,7 +66,10 @@ def normalize
         clause
   | _ => clause
 
-private def clauseParser : P Clause :=
+private
+def clauseParser
+    : P Clause
+    :=
   GParser.fix fun recursive =>
     let parenthesized : P Clause :=
       GParser.ch '(' *> trivia *> recursive <* GParser.ch ')' <* trivia
